Poe.lean
@@ -1,5 +1,6 @@
 import Poe.Uplc
 import Poe.Emit
+import Poe.Prelude
 import Poe.Translate
 import Poe.Oracle
 import Poe.Lint
